Axiomatic construction of Operational Semantics for [row]

theories/Row.v
@@ -1,11 +1,27 @@
 Require Import FreeSpec.Interface.
 Require Import FreeSpec.Open.
 Require Import FreeSpec.Control.
+Require Import FreeSpec.Control.Option.
 Require Import FreeSpec.Program.
+Require Import FreeSpec.Semantics.
 
 Require Import Coq.Lists.List.
 
 Local Open Scope free_control_scope.
+
+Polymorphic Fixpoint getr
+            (set:  list (Type -> Type))
+            (n:    nat)
+            {struct n}
+  : Type -> Type :=
+  match n, set with
+  | 0, t :: _
+    => t
+  | S n, _ :: set'
+    => getr set' n
+  | _, _
+    => fun _ => inhabited
+  end.
 
 Fixpoint specialize
          (x:    Type)
@@ -18,6 +34,17 @@ Fixpoint specialize
     => nil
   end.
 
+Fixpoint generalize
+         (x:    (Type -> Type) -> Type)
+         (row:  list (Type -> Type))
+  : list Type :=
+  match row with
+  | i :: rest
+    => x i :: generalize x rest
+  | nil
+    => nil
+  end.
+
 Inductive row
           (set:  list (Type -> Type))
           (a:    Type)
@@ -25,11 +52,15 @@ Inductive row
 | Row (e:  union (specialize a set))
   : row set a.
 
+Arguments Row [set a] (e).
+
 Class HasEffect
       (set:  list (Type -> Type))
       (I:    Type -> Type)
-  := { contains_effects :> forall (r:  Type),
+  := { contains_spec :> forall (r:  Type),
            Contains (I r) (specialize r set)
+     ; contains_gen :> forall (f: (Type -> Type) -> Type),
+           Contains (f I) (generalize f set)
      }.
 
 Instance HasEffect_head
@@ -52,7 +83,7 @@ Definition inj_effect
            {set:  list (Type -> Type)} `{HasEffect set I}
            (x:    I a)
   : Program (row set) a :=
-  Request (Row set a (inj (set := specialize a set) x)).
+  Request (Row (inj (set := specialize a set) x)).
 
 Section EXAMPLE.
   Inductive E1
@@ -73,3 +104,47 @@ Section EXAMPLE.
     x <- inj_effect e1;
     inj_effect (e2 x).
 End EXAMPLE.
+
+Fact get_spec_getr_eq
+     (set:  list (Type -> Type))
+     (a:    Type)
+     (n:    nat)
+  : get (specialize a set) n = (getr set n) a.
+Proof.
+  revert n.
+  induction set; intros n.
+  + cbn.
+    induction n; reflexivity.
+  + induction n; [ reflexivity |].
+    cbn in *.
+    apply IHset.
+Qed.
+
+Instance HasEffect_indexed
+         (set:  list (Type -> Type))
+         (n:    nat)
+  : HasEffect set (getr set n) :=
+  {}.
+Admitted.
+
+Definition semanticsRowSteps
+           (set:   list (Type -> Type))
+  : @PS (row set) (product (generalize Semantics set)).
+  unfold PS.
+  intros a sems e.
+  refine (
+      match e with
+      | Row (OneOf n Ht x)
+        => _
+      end
+    ).
+  rewrite get_spec_getr_eq in Ht.
+  subst.
+  exact (visit sems (fun s => handle s x)).
+Defined.
+
+Definition mkSemanticsForRow
+           {set:  list (Type -> Type)}
+           (sems:  product (generalize Semantics set))
+  : Semantics (row set) :=
+  mkSemantics (semanticsRowSteps set) sems.
